src/single_conf_message/DY.Example.SingleConfMessage.SecurityProperties.fst
@@ -10,17 +10,13 @@ open DY.Example.SingleConfMessage.Protocol.Stateful.Proof
 
 #set-options "--fuel 0 --ifuel 0 --z3rlimit 10  --z3cliopt 'smt.qi.eager_threshold=100'"
 
-// This is the main security property of a
-// confidential message. It states from the sender
-// perspective that the secret is not leaked to
-// the attacker as long as the sender and receiver
-// are honest.
+// This is the main security property of a confidential message. It states from
+// the sender perspective that the secret is not leaked to the attacker as long
+// as the sender and receiver are honest.
 //
-// **Note:** We know that if the receiver is
-// honest only the receiver can decrypt the
-// secret. This allows us to argue from the
-// sender's perspective that if the attacker knows
-// the secret either the sender or the receiver is
+// **Note:** We know that if the receiver is honest only the receiver can
+// decrypt the secret. This allows us to argue from the sender's perspective
+// that if the attacker knows the secret either the sender or the receiver is
 // corrupt.
 val secret_secrecy_sender:
   tr:trace -> sender:principal -> receiver:principal -> msg:single_message ->
@@ -37,10 +33,9 @@ let secret_secrecy_sender tr sender receiver msg =
   attacker_only_knows_publishable_values tr msg.secret;
   ()
 
-// On the receiver side we don't have any
-// guarantees on the secrecy of the secret. We can
-// only prove that if the attacker knows the
-// secret, it is publishable.
+// On the receiver side we don't have any guarantees on the secrecy of the
+// secret. We can only prove that if the attacker knows the secret, it is
+// publishable.
 val secret_secrecy_receiver:
   tr:trace -> sender:principal -> receiver:principal -> secret:bytes ->
   Lemma
@@ -55,11 +50,9 @@ let secret_secrecy_receiver tr sender receiver secret =
   attacker_only_knows_publishable_values tr secret;
   ()
 
-// We can also not authenticate the sender because
-// the attacker could write an arbitrary sender in
-// the message. The only thing we can prove is
-// that if the secret is not publisable, there
-// exists a sender that triggered the send event.
+// We can also not authenticate the sender because the attacker could have
+// encrypted the message The only thing we can prove is that if the secret is
+// not publisable, there exists a sender that triggered the send event.
 val sender_authentication:
   tr:trace ->
   receiver:principal ->
@@ -71,13 +64,10 @@ val sender_authentication:
   )
   (ensures
     (exists sender. event_triggered tr sender (SenderSendMsg sender receiver msg)) \/
-    is_publishable tr (compute_message msg.secret)
-    // We cannot prove `is_corrupt tr
-    // (principal_label sender)` because the
-    // sender is not authenticated. If the
-    // attacker creates this message, they can
-    // choose an arbitrary sender for the sender
-    // field.
+    is_publishable tr (serialize single_message msg)
+    // We cannot prove `is_corrupt tr (principal_label sender)` because the
+    // sender is not authenticated. If the attacker creates this message, they
+    // can choose an arbitrary sender for the sender field.
   )
 let sender_authentication tr receiver secret = ()
 
@@ -86,7 +76,6 @@ let sender_authentication tr receiver secret = ()
 // This is not provable because the receiver event
 // is in the future, and it is not guaranteed that
 // it is ever triggered.
-
 val recever_authentication:
   tr:trace ->
   sender:principal -> receiver:principal ->
